proofs/hol_light/aarch64/proofs/mldsa_pointwise_montgomery_aarch64_asm.ml
@@ -72,13 +72,13 @@ let mldsa_pointwise_mc = define_assert_from_elf
 ];;
 (*** BYTECODE END ***)
 
-let MLDSA_POINTWISE_EXEC = ARM_MK_EXEC_RULE mldsa_pointwise_mc;;
+let MLDSA_POINTWISE_MONTGOMERY_EXEC = ARM_MK_EXEC_RULE mldsa_pointwise_mc;;
 
 (* ========================================================================= *)
 (* Correctness proof                                                         *)
 (* ========================================================================= *)
 
-let MLDSA_POINTWISE_CORRECT = prove
+let MLDSA_POINTWISE_MONTGOMERY_CORRECT = prove
  (`!a b x y pc.
     nonoverlapping (word pc, LENGTH mldsa_pointwise_mc) (a, 1024) /\
     nonoverlapping (a, 1024) (b, 1024)
@@ -107,7 +107,7 @@ let MLDSA_POINTWISE_CORRECT = prove
      `x:num->int32`; `y:num->int32`; `pc:num`] THEN
   REWRITE_TAC[MAYCHANGE_REGS_AND_FLAGS_PERMITTED_BY_ABI; C_ARGUMENTS;
               NONOVERLAPPING_CLAUSES; ALL;
-              fst MLDSA_POINTWISE_EXEC] THEN
+              fst MLDSA_POINTWISE_MONTGOMERY_EXEC] THEN
   DISCH_THEN(REPEAT_TCL CONJUNCTS_THEN ASSUME_TAC) THEN
   GLOBALIZE_PRECONDITION_TAC THEN
   CONV_TAC(RATOR_CONV(LAND_CONV(ONCE_DEPTH_CONV EXPAND_CASES_CONV))) THEN
@@ -126,7 +126,7 @@ let MLDSA_POINTWISE_CORRECT = prove
   DISCARD_MATCHING_ASSUMPTIONS [`read (memory :> bytes32 a) s = x`] THEN
 
   (* Simulate all 679 instructions with SIMD simplification *)
-  MAP_EVERY (fun n -> ARM_STEPS_TAC MLDSA_POINTWISE_EXEC [n] THEN
+  MAP_EVERY (fun n -> ARM_STEPS_TAC MLDSA_POINTWISE_MONTGOMERY_EXEC [n] THEN
                       SIMD_SIMPLIFY_TAC[arm_mldsa_pointwise_montred'])
         (1--679) THEN
   ENSURES_FINAL_STATE_TAC THEN ASM_REWRITE_TAC[] THEN
@@ -209,7 +209,7 @@ let MLDSA_POINTWISE_CORRECT = prove
 (* Subroutine form                                                           *)
 (* ========================================================================= *)
 
-let MLDSA_POINTWISE_SUBROUTINE_CORRECT = prove
+let MLDSA_POINTWISE_MONTGOMERY_SUBROUTINE_CORRECT = prove
  (`!a b x y pc returnaddress.
     nonoverlapping (word pc, LENGTH mldsa_pointwise_mc) (a, 1024) /\
     nonoverlapping (a, 1024) (b, 1024)
@@ -232,9 +232,9 @@ let MLDSA_POINTWISE_SUBROUTINE_CORRECT = prove
                  abs(ival zi) <= &8380416))
           (MAYCHANGE_REGS_AND_FLAGS_PERMITTED_BY_ABI ,,
            MAYCHANGE [memory :> bytes(a, 1024)])`,
-  REWRITE_TAC[fst MLDSA_POINTWISE_EXEC] THEN
-  ARM_ADD_RETURN_NOSTACK_TAC MLDSA_POINTWISE_EXEC
-    (REWRITE_RULE[fst MLDSA_POINTWISE_EXEC] MLDSA_POINTWISE_CORRECT));;
+  REWRITE_TAC[fst MLDSA_POINTWISE_MONTGOMERY_EXEC] THEN
+  ARM_ADD_RETURN_NOSTACK_TAC MLDSA_POINTWISE_MONTGOMERY_EXEC
+    (REWRITE_RULE[fst MLDSA_POINTWISE_MONTGOMERY_EXEC] MLDSA_POINTWISE_MONTGOMERY_CORRECT));;
 
 (* ========================================================================= *)
 (* Constant-time and memory safety proof.                                    *)
@@ -246,10 +246,10 @@ needs "mldsa_native/aarch64/proofs/subroutine_signatures.ml";;
 let full_spec,public_vars = mk_safety_spec
     ~keep_maychanges:false
     (assoc "mldsa_pointwise" subroutine_signatures)
-    MLDSA_POINTWISE_SUBROUTINE_CORRECT
-    MLDSA_POINTWISE_EXEC;;
+    MLDSA_POINTWISE_MONTGOMERY_SUBROUTINE_CORRECT
+    MLDSA_POINTWISE_MONTGOMERY_EXEC;;
 
-let MLDSA_POINTWISE_SUBROUTINE_SAFE = time prove
+let MLDSA_POINTWISE_MONTGOMERY_SUBROUTINE_SAFE = time prove
  (`exists f_events.
        forall e a b pc returnaddress.
            nonoverlapping (word pc,LENGTH mldsa_pointwise_mc) (a,1024) /\
@@ -271,4 +271,4 @@ let MLDSA_POINTWISE_SUBROUTINE_SAFE = time prove
                          [a,1024]))
                (\s s'. true)`,
   ASSERT_CONCL_TAC full_spec THEN
-  PROVE_SAFETY_SPEC_TAC ~public_vars:public_vars MLDSA_POINTWISE_EXEC);;
+  PROVE_SAFETY_SPEC_TAC ~public_vars:public_vars MLDSA_POINTWISE_MONTGOMERY_EXEC);;
